@prefix : <https://nfdi4culture.de/ontology#> .
@prefix owl: <http://www.w3.org/2002/07/owl#> .
@prefix rdf: <http://www.w3.org/1999/02/22-rdf-syntax-ns#> .
@prefix xml: <http://www.w3.org/XML/1998/namespace> .
@prefix xsd: <http://www.w3.org/2001/XMLSchema#> .
@prefix rdfs: <http://www.w3.org/2000/01/rdf-schema#> .
@base <https://nfdi4culture.de/ontology#> .

<https://nfdi4culture.de/ontology#> rdf:type owl:Ontology ;
                                     <http://purl.org/dc/elements/1.1/creator> <https://nfdi4culture.de/id/E1925> ,
                                                                               <https://nfdi4culture.de/id/E2415> ,
                                                                               <https://nfdi4culture.de/id/E2416> ,
                                                                               <https://nfdi4culture.de/id/E3095> ;
                                     <http://purl.org/dc/elements/1.1/title> "NFDI4Culture Ontology" ;
                                     <http://purl.org/dc/terms/abstract> """The NFDI4Culture ontology (CTO) is an ontology for the representation and categorization of various resources within the domain of NFDI4Culture. It encompasses a wide array of entities including datasets, individual items and cultural heritage objects, data providers, persons, projects, and other pertinent elements relevant to cultural heritage and research endeavors. CTO is a module that builds upon the NFDIcore Ontology (https://ise-fizkarlsruhe.github.io/nfdicore/). With the advent of version v.2.2.0, CTO is aligned with NFDIcore v.2.0.0 and its subsequent versions, while ensuring compatibility with the Basic Formal Ontology (BFO).

At its core, the ontology provides a structured means to describe and connect diverse entities, facilitating efficient organization, retrieval, and analysis of cultural data. By defining classes such as cto:DatafeedElement, cto:Item, it establishes clear distinctions and relationships between different types of resources, enabling nuanced classification and enhanced comprehension of the domain.

Moreover, the ontology incorporates essential properties and relationships, such as cto:elementOf, nfdicore:publisher, nfdicore:license, and cto:temporalCoverage, to enrich the descriptions of resources and provide additional contextual information and intrconnection of elements across culture disciplines. This ensures a more robust representation of cultural artifacts, datasets, and associated metadata, thereby supporting a wide range of scholarly and practical applications within the NFDI4Culture ecosystem."""@en ;
                                     <http://purl.org/dc/terms/bibliographicCitation> "Oleksandra Bruns, Tabea Tietz, Etienne Posthumus, Harald Sack. NFDI4Culture Ontology. Revision: v2.2.0. Retrieved from:"^^rdfs:Literal ;
                                     <http://purl.org/dc/terms/hasVersion> "v2.2.0"^^rdfs:Literal ;
                                     <http://purl.org/vocab/vann/preferredNamespacePrefix> "cto"^^rdfs:Literal ;
                                     <http://purl.org/vocab/vann/preferredNamespaceUri> <https://creativecommons.org/publicdomain/zero/1.0/> ,
                                                                                        <https://nfdi4culture.de/ontology#> ;
                                     rdfs:label "NFDI4Culture Ontology (cto)" ;
                                     rdfs:seeAlso <https://nfdi4culture.de/ontology.json> ,
                                                  <https://nfdi4culture.de/ontology.nt> ,
                                                  <https://nfdi4culture.de/ontology.rdf> ,
                                                  <https://nfdi4culture.de/ontology.ttl> ,
                                                  <https://nfdi4culture.de/ontology/about.html> ;
                                     owl:priorVersion "2.1"^^rdfs:Literal ;
                                     owl:versionInfo "v.2.2.0" .

#################################################################
#    Annotation properties
#################################################################

###  http://purl.org/dc/elements/1.1/creator
<http://purl.org/dc/elements/1.1/creator> rdf:type owl:AnnotationProperty .


###  http://purl.org/dc/elements/1.1/title
<http://purl.org/dc/elements/1.1/title> rdf:type owl:AnnotationProperty .


###  http://purl.org/dc/terms/abstract
<http://purl.org/dc/terms/abstract> rdf:type owl:AnnotationProperty .


###  http://purl.org/dc/terms/bibliographicCitation
<http://purl.org/dc/terms/bibliographicCitation> rdf:type owl:AnnotationProperty .


###  http://purl.org/dc/terms/hasVersion
<http://purl.org/dc/terms/hasVersion> rdf:type owl:AnnotationProperty .


###  http://purl.org/dc/terms/license
<http://purl.org/dc/terms/license> rdf:type owl:AnnotationProperty .


###  http://purl.org/vocab/vann/preferredNamespacePrefix
<http://purl.org/vocab/vann/preferredNamespacePrefix> rdf:type owl:AnnotationProperty .


###  http://purl.org/vocab/vann/preferredNamespaceUri
<http://purl.org/vocab/vann/preferredNamespaceUri> rdf:type owl:AnnotationProperty .


###  https://nfdi.fiz-karlsruhe.de/ontology/example
<https://nfdi.fiz-karlsruhe.de/ontology/example> rdf:type owl:AnnotationProperty .


#################################################################
#    Datatypes
#################################################################

###  http://www.w3.org/2001/XMLSchema#date
xsd:date rdf:type rdfs:Datatype .


#################################################################
#    Object Properties
#################################################################

###  http://purl.org/dc/terms/isPartOf
<http://purl.org/dc/terms/isPartOf> rdf:type owl:ObjectProperty ;
                                    owl:equivalentProperty <http://schema.org/isPartOf> ;
                                    rdfs:domain <https://nfdi.fiz-karlsruhe.de/ontology/Resource> ;
                                    rdfs:range <https://nfdi.fiz-karlsruhe.de/ontology/Resource> ;
                                    rdfs:comment "This property establishes a connection between a resource and the overarching resource to which it belongs, e.g. an individual item to the dataset it is part of."@en .


###  http://purl.org/ontology/mo/lyrics
<http://purl.org/ontology/mo/lyrics> rdf:type owl:ObjectProperty ;
                                     rdfs:domain <http://purl.org/ontology/mo/MusicalWork> ;
                                     rdfs:range <http://purl.org/ontology/mo/Lyrics> ;
                                     rdfs:comment "This property establishes a connection between a resource of type musical work and a lyrics entity."@en .


###  http://schema.org/image
<http://schema.org/image> rdf:type owl:ObjectProperty ;
                          rdfs:domain :DatafeedElement ;
                          rdfs:range owl:Thing .


###  http://schema.org/isPartOf
<http://schema.org/isPartOf> rdf:type owl:ObjectProperty .


###  http://schema.org/url
<http://schema.org/url> rdf:type owl:ObjectProperty .


###  https://nfdi4culture.de/ontology#aat
:aat rdf:type owl:ObjectProperty ;
     rdfs:subPropertyOf :externalVocabulary ;
     rdfs:domain <http://schema.org/CreativeWork> ;
     rdfs:range owl:Thing ;
     rdfs:comment "The property relates a creative work resource to a concept, term, or classification type in Art & Architecture Thesaurus."@en ;
     rdfs:label "AAT"@en ;
     <https://nfdi.fiz-karlsruhe.de/ontology/example> "A stained glass window artwork \"Engel mit Dudelsack\" has a related AAT entry <http://vocab.getty.edu/page/aat/300263722>"@en .


###  https://nfdi4culture.de/ontology#ddbAPI
:ddbAPI rdf:type owl:ObjectProperty ;
        rdfs:subPropertyOf <http://schema.org/url> ;
        rdfs:domain <https://nfdi.fiz-karlsruhe.de/ontology/Resource> ;
        rdfs:range owl:Thing ;
        rdfs:comment "The property relates the resource to the DDB API Endpoint associated with the resource."@en ;
        rdfs:label "DDB API"^^rdfs:Literal ;
        <https://nfdi.fiz-karlsruhe.de/ontology/example> "https://api.deutsche-digitale-bibliothek.de/items/OUOATUXI6I7XMWYRRKAXGXGEM3E6JD3D/source/record"^^rdfs:Literal .


###  https://nfdi4culture.de/ontology#elementOf
:elementOf rdf:type owl:ObjectProperty ;
           rdfs:subPropertyOf <http://purl.org/dc/terms/isPartOf> ;
           rdfs:domain :DatafeedElement ;
           rdfs:range <https://nfdi.fiz-karlsruhe.de/ontology/Resource> ;
           rdfs:comment "This property connects an element and the overarching resource it belongs to, e.g. an individual item and the dataset it is part of."@en ;
           rdfs:label "element of"@en ;
           <https://nfdi.fiz-karlsruhe.de/ontology/example> "\"Engel mit Dudelsack\" is a single element in the digital image dataset Corpus Vitrearum Medii Aevi Deutschland"@en .


###  https://nfdi4culture.de/ontology#elementType
:elementType rdf:type owl:ObjectProperty ;
             rdfs:domain :DatafeedElement ;
             rdfs:range owl:Thing ;
             rdfs:comment """The property is recommended to be used in combination with the subproperties of cto:externalVocabulary to specify the vocabulary the element type is defined with:

For example:
<:Frühlingsgruß   cto:elementType <https://rism.online/subjects/25227>>
<:Frühlingsgruß   cto:rism <https://rism.online/subjects/25227>>"""@en ,
                          "The property relates a datafeed element to its category within a predefined vocabulary/taxonomy, indicating the nature or genre of the element. The type must be taken from a published controlled vocabulary, e.g. AAT, GND, Wikidata, Iconclass, FactGrid, etc."@en ;
             rdfs:label "element type"@en ;
             <https://nfdi.fiz-karlsruhe.de/ontology/example> """http://vocab.getty.edu/aat/300003725 (altars (religious fixtures))
http://vocab.getty.edu/aat/300047090 (sculpture (visual works))
https://www.wikidata.org/wiki/Q101687 (altar)"""^^rdfs:Literal .


###  https://nfdi4culture.de/ontology#externalVocabulary
:externalVocabulary rdf:type owl:ObjectProperty ;
                    rdfs:domain owl:Thing ;
                    rdfs:range owl:Thing ;
                    rdfs:comment """The property and its subproperties are recommended to be used in combination with:

cto:elementType
cto:subjectConcept
cto:relatedPerson
cto:relatedLocation

For example:
<:Frühlingsgruß   cto:rism <https://rism.online/subjects/25227>>
<:Frühlingsgruß   cto:elementType <https://rism.online/subjects/25227>>"""@en ,
                                 "This property establishes a connection between a thing and an external controlled vocabulary, providing additional semantic information from external sources. The subproperties of cto:externalVocabulary should be used for standard reference systems such as AAT, GeoNames, GND, Iconclass, Wikidata, RISM."@en ;
                    rdfs:label "external vocabulary"@en .


###  https://nfdi4culture.de/ontology#factgrid
:factgrid rdf:type owl:ObjectProperty ;
          rdfs:subPropertyOf :externalVocabulary ;
          rdfs:domain owl:Thing ;
          rdfs:range owl:Thing ;
          rdfs:comment "Adolph Freiherr Knigge has element type \"Human\" (<https://database.factgrid.de/wiki/Item:Q7>) in FactGrid database."@en ,
                       "The property relates a thing to a concept, term, or classification type in FactGrid database."@en ;
          rdfs:label "FactGrid"@en .


###  https://nfdi4culture.de/ontology#geonames
:geonames rdf:type owl:ObjectProperty ;
          rdfs:subPropertyOf :externalVocabulary ;
          rdfs:domain owl:Thing ;
          rdfs:range owl:Thing ;
          rdfs:comment "The property relates a thing to a location in the GeoNames geographical database."@en ;
          rdfs:label "GeoNames"@en ;
          <https://nfdi.fiz-karlsruhe.de/ontology/example> "A stained glass window artwork \"Engel mit Dudelsack\" has a related GeoNames location <http://sws.geonames.org/11427995>"@en .


###  https://nfdi4culture.de/ontology#gnd
:gnd rdf:type owl:ObjectProperty ;
     rdfs:subPropertyOf :externalVocabulary ;
     rdfs:domain owl:Thing ;
     rdfs:range owl:Thing ;
     rdfs:comment "The property relates a thing to the corresponding entry or related concept of the thing in GND (Integrated Authority File)."@en ;
     rdfs:label "GND"@en ;
     <https://nfdi.fiz-karlsruhe.de/ontology/example> "A caricature image \"Gedichte eines Kleinstädters\" has a related GND entry <https://d-nb.info/gnd/118680609>"@en .


###  https://nfdi4culture.de/ontology#iconclass
:iconclass rdf:type owl:ObjectProperty ;
           rdfs:subPropertyOf :externalVocabulary ;
           rdfs:domain <http://schema.org/CreativeWork> ;
           rdfs:range owl:Thing ;
           rdfs:comment "The property relates a creative work to the subject concept or content of the creative work in the Iconclass classification system."@en ;
           rdfs:label "Iconclass"@en ;
           <https://nfdi.fiz-karlsruhe.de/ontology/example> "A stained glass window artwork \"Engel mit Dudelsack\" has a related Iconclass entry <https://iconclass.org/11G21>"@en .


###  https://nfdi4culture.de/ontology#iiifImageAPI
:iiifImageAPI rdf:type owl:ObjectProperty ;
              rdfs:subPropertyOf <http://schema.org/url> ;
              rdfs:domain :DatafeedElement ;
              rdfs:range owl:Thing ;
              rdfs:comment "The property relates the datafeed element to the IIIF Image API associated with the image of the element."@en ;
              rdfs:label "IIIF Image API"^^rdfs:Literal ;
              <https://nfdi.fiz-karlsruhe.de/ontology/example> "https://heidicon.ub.uni-heidelberg.de/iiif/2/2305%3A2123"^^rdfs:Literal .


###  https://nfdi4culture.de/ontology#iiifPresentationAPI
:iiifPresentationAPI rdf:type owl:ObjectProperty ;
                     rdfs:subPropertyOf <http://schema.org/url> ;
                     rdfs:domain :DatafeedElement ;
                     rdfs:range owl:Thing ;
                     rdfs:comment "The property relates the datafeed element to the IIIF Presentation API associated with the element."@en ;
                     rdfs:label "IIIF Presentation API"^^rdfs:Literal ;
                     <https://nfdi.fiz-karlsruhe.de/ontology/example> "https://heidicon.ub.uni-heidelberg.de/iiif/2/597256:51961/info.json"@en .


###  https://nfdi4culture.de/ontology#incipitOf
:incipitOf rdf:type owl:ObjectProperty ;
           rdfs:subPropertyOf <http://purl.org/dc/terms/isPartOf> ;
           rdfs:domain :Incipit ;
           rdfs:range <http://schema.org/MusicComposition> ;
           rdfs:comment "The property connects an incipit and the music composition it belongs to."@en ;
           rdfs:label "incipit of"@en ;
           <https://nfdi.fiz-karlsruhe.de/ontology/example> "https://rism.online/sources/201001959/incipits/1.1.1 is an incipit of musical composition \"Frühlingsgruß\" (https://rism.online/sources/201001959) by Robert Schumann."@en .


###  https://nfdi4culture.de/ontology#oai-pmhAPI
:oai-pmhAPI rdf:type owl:ObjectProperty ;
            rdfs:subPropertyOf <http://schema.org/url> ;
            rdfs:domain <https://nfdi.fiz-karlsruhe.de/ontology/Resource> ;
            rdfs:range owl:Thing ;
            rdfs:comment "The property relates the resource to the OAI-PMH API Endpoint associated with the resource."@en ;
            rdfs:label "OAI-PMH API"^^rdfs:Literal ;
            <https://nfdi.fiz-karlsruhe.de/ontology/example> "https://heidicon.ub.uni-heidelberg.de/api/v1/plugin/base/oai/oai?verb=GetRecord&metadataPrefix=lido&identifier=oai:heidicon.ub.uni-heidelberg.de:ed84679c-e602-4b7c-9e77-f8b5c9c97b74"^^rdfs:Literal .


###  https://nfdi4culture.de/ontology#relatedEvent
:relatedEvent rdf:type owl:ObjectProperty ;
              rdfs:domain :DatafeedElement ;
              rdfs:range <https://nfdi.fiz-karlsruhe.de/ontology/Event> ;
              rdfs:comment "The property establishes a connection between an element and the diverse events associated with the described datafeed element, which may include attendance, hosting, performance, sponsorship, or collaboration, contributing, witnessing, etc. of a specific event."@en ,
                           """The property is recommended to be used in combination with the subproperties of cto:externalVocabulary to explicitly indicate the vocabulary through which the event related to the element is defined:

For example:
<:AdolphFreiherrKnigge cto:relatedEvent <https://database.factgrid.de/entity/Q23430>>
<:AdolphFreiherrKnigge cto:factgrid <https://database.factgrid.de/entity/Q23430>>"""@en ;
              rdfs:label "related event"@en .


###  https://nfdi4culture.de/ontology#relatedItem
:relatedItem rdf:type owl:ObjectProperty ;
             rdfs:domain :DatafeedElement ;
             rdfs:range :Item ;
             rdfs:comment """The property is recommended to be used in combination with the subproperties of cto:externalVocabulary to explicitly indicate the vocabulary through which the item related to the element is defined:

For example:
<:AdolphFreiherrKnigge cto:relatedItem <https://database.factgrid.de/entity/Q12913>>
<:AdolphFreiherrKnigge cto:factgrid <https://database.factgrid.de/entity/Q12913>>"""@en ,
                          "The property relates a datafeed element to an item it is related to."@en ;
             rdfs:label "related item"@en .


###  https://nfdi4culture.de/ontology#relatedLocation
:relatedLocation rdf:type owl:ObjectProperty ;
                 rdfs:domain :DatafeedElement ;
                 rdfs:range <https://nfdi.fiz-karlsruhe.de/ontology/Place> ;
                 rdfs:comment """The property establishes a connection between an element and the locations that are associated with the described datafeed element. These locations may include the physical location of the item, the geographical setting depicted in the item, the locations explicitly mentioned or implied within the item's content, the birth or death places of a person, the location of an event, etc. The locations must be taken from a published controlled vocabulary, e.g. GND, Wikidata, GeoNames.

In contrast to nfdicore:location, it covers broader aspects of locations associated with an element, including physical, geographical, and content-related locations. Additionally, it enforces the use of a controlled vocabulary for specifying these locations."""@en ,
                              """The property is recommended to be used in combination with the subproperties of cto:externalVocabulary to specify the vocabulary the location related to the element is defined with:

For example:
<:EngelMitDudelsack   cto:relatedLocation <http://sws.geonames.org/11427995>>
<:EngelMitDudelsack   cto:geonames <http://sws.geonames.org/11427995>>"""@en ;
                 rdfs:label "related location"@en ;
                 <https://nfdi.fiz-karlsruhe.de/ontology/example> """https://sws.geonames.org/2950159/ (Berlin)
https://www.wikidata.org/wiki/Q64 (Berlin)"""^^rdfs:Literal .


###  https://nfdi4culture.de/ontology#relatedOrganization
:relatedOrganization rdf:type owl:ObjectProperty ;
                     rdfs:domain :DatafeedElement ;
                     rdfs:range <https://nfdi.fiz-karlsruhe.de/ontology/Organization> ;
                     rdfs:comment """The property is recommended to be used in combination with the subproperties of cto:externalVocabulary to explicitly indicate the vocabulary through which the organization related to the element is defined:

For example:
<:AdolphFreiherrKnigge cto:relatedOrganization <https://database.factgrid.de/entity/Q81288>>
<:AdolphFreiherrKnigge cto:factgrid <https://database.factgrid.de/entity/Q81288>>"""@en ,
                                  "The property links an element to the various organizations affiliated with the described datafeed element. These organizations encompass a diverse range, such as educational institutions, workplaces, interest groups, event organizers, etc. The organizations must be taken from a published controlled vocabulary, e.g. GND, Wikidata, FactGrid."@en ;
                     rdfs:label "related organization"@en .


###  https://nfdi4culture.de/ontology#relatedPerson
:relatedPerson rdf:type owl:ObjectProperty ;
               rdfs:domain :DatafeedElement ;
               rdfs:range <https://nfdi.fiz-karlsruhe.de/ontology/Person> ;
               rdfs:comment """The property is recommended to be used in combination with the subproperties of cto:externalVocabulary to explicitly indicate the vocabulary through which the person related to the datafeed element is defined:

For example:
<:WasIhrWollt cto:relatedPerson <http://www.wikidata.org/entity/Q692>>
<:WasIhrWollt cto:wikidata <http://www.wikidata.org/entity/Q692>>"""@en ,
                            "The property relates an element to individuals associated with the described element. These individuals may include item creators, set/costume designers, actors, addressers, performers, relatives, friends, event participants, etc. The individuals must be taken from a published controlled vocabulary, e.g. GND, Wikidata."@en ;
               rdfs:label "related person"@en ;
               <https://nfdi.fiz-karlsruhe.de/ontology/example> """https://www.wikidata.org/wiki/Q34628 (Gotthold Ephraim Lessing)
https://d-nb.info/gnd/142585777 (Wilke, Insa)"""@en .


###  https://nfdi4culture.de/ontology#rism
:rism rdf:type owl:ObjectProperty ;
      rdfs:subPropertyOf :externalVocabulary ;
      rdfs:domain <http://purl.org/ontology/mo/MusicalWork> ;
      rdfs:range owl:Thing ;
      rdfs:comment "The property relates a musical item to the corresponding entry or related concept of the item in RISM (Répertoire International des Sources Musicales)."@en ;
      rdfs:label "RISM"@en ;
      <https://nfdi.fiz-karlsruhe.de/ontology/example> "A musical composition \"Frühlingsgruß\" has a related RISM entry <https://rism.online/subjects/25227>"@en .


###  https://nfdi4culture.de/ontology#sourceFile
:sourceFile rdf:type owl:ObjectProperty ;
            rdfs:subPropertyOf <http://schema.org/url> ;
            rdfs:domain <https://nfdi.fiz-karlsruhe.de/ontology/Resource> ;
            rdfs:range owl:Thing ;
            rdfs:comment "The property links a resource to the URL of a data source from which it originates, e.g. in an API endpoint."@en ;
            rdfs:label "source file"^^rdfs:Literal ;
            <https://nfdi.fiz-karlsruhe.de/ontology/example> "https://heidicon.ub.uni-heidelberg.de/api/v1/plugin/base/oai/oai?verb=GetRecord&metadataPrefix=lido&identifier=oai:heidicon.ub.uni-heidelberg.de:ed84679c-e602-4b7c-9e77-f8b5c9c97b74"^^rdfs:Literal .


###  https://nfdi4culture.de/ontology#subjectConcept
:subjectConcept rdf:type owl:ObjectProperty ;
                rdfs:domain :DatafeedElement ;
                rdfs:range owl:Thing ;
                rdfs:comment """The property is recommended to be used in combination with the subproperties of cto:externalVocabulary to specify the vocabulary the subject concept is defined with:

For example:
<:EngelMitDudelsack   cto:subjectConcept <https://iconclass.org/11G21>>
<:EngelMitDudelsack   cto:iconclass <https://iconclass.org/11G21>>"""@en ,
                             "The property relates an element to concepts related to the subject of the element within a predefined vocabulary/taxonomy. It may be used to associate the item with specific ideas, themes, or topics, e.g. iconography, themes from literature, terms, concepts, related works that item is based on, domain of interest of a person, theme of the event, etc. The subject must be taken from a published controlled vocabulary, e.g. AAT, GND, Wikidata, Iconclass."@en ;
                rdfs:label "subject concept"@en ;
                <https://nfdi.fiz-karlsruhe.de/ontology/example> """http://iconclass.org/11H (saints)
https://iconclass.org/11K (devil(s) and demons)
https://www.wikidata.org/wiki/Q581450 (fallen angel)
https://d-nb.info/gnd/4099291-3 (Minna von Barnhelm)"""@en .


###  https://nfdi4culture.de/ontology#viaf
:viaf rdf:type owl:ObjectProperty ;
      rdfs:subPropertyOf :externalVocabulary ;
      rdfs:domain owl:Thing ;
      rdfs:range owl:Thing ;
      rdfs:comment "The property relates a thing to the corresponding entry in VIAF: Virtual International Authority File."@en ;
      rdfs:label "VIAF"@en ;
      <https://nfdi.fiz-karlsruhe.de/ontology/example> "Robert Schumann has a corresponding VIAF entity <https://viaf.org/viaf/7575259>"@en .


###  https://nfdi4culture.de/ontology#wikidata
:wikidata rdf:type owl:ObjectProperty ;
          rdfs:subPropertyOf :externalVocabulary ;
          rdfs:domain owl:Thing ;
          rdfs:range owl:Thing ;
          rdfs:comment "The property relates a thing to the corresponding entry or related concept of the item in Wikidata."@en ;
          rdfs:label "Wikidata"@en ;
          <https://nfdi.fiz-karlsruhe.de/ontology/example> "A theatrical performance of \"Was ihr Wollt\" has a related Wikidata entry <http://www.wikidata.org/entity/Q221211>"@en .


#################################################################
#    Data properties
#################################################################

###  http://purl.org/ontology/mo/text
<http://purl.org/ontology/mo/text> rdf:type owl:DatatypeProperty ;
                                   rdfs:domain <http://purl.org/ontology/mo/Lyrics> ;
                                   rdfs:range rdfs:Literal ;
                                   rdfs:comment "The property relates the lyrics entity of a musical work and its text." .


###  http://schema.org/temporalCoverage
<http://schema.org/temporalCoverage> rdf:type owl:DatatypeProperty ;
                                     rdfs:comment "The generic property that relates an item to its broad temporal attributes, e.g. the period of its existence, the dates of the creation, destruction, and approximate dates."@en ,
                                                  "Use related properties e.g. nfdcore:birthDate, nfdicore:deathDate for describing Persons, or nfdicore:startDate, nfdicore:endDate for describing Events."@en .


###  https://nfdi4culture.de/ontology#approximatePeriod
:approximatePeriod rdf:type owl:DatatypeProperty ;
                   rdfs:subPropertyOf <http://schema.org/temporalCoverage> ;
                   rdfs:domain :Item ;
                   rdfs:range rdfs:Literal ;
                   rdfs:comment "The property relates an item to the approximate time the item is associated with. It often links to time periods/dates containing temporal constraints, e.g. \"during, before, after\" to approximate the time. The property should only be used to express an estimated or imprecise date associated with an item when the exact date is uncertain or not precisely known."@en ;
                   rdfs:label "approximate period"@en ;
                   <https://nfdi.fiz-karlsruhe.de/ontology/example> "\"vor 1397\", \"nach 15 Jahrhundert\""^^rdfs:Literal .


###  https://nfdi4culture.de/ontology#clef
:clef rdf:type owl:DatatypeProperty ;
      rdfs:domain :Incipit ;
      rdfs:range rdfs:Literal ;
      rdfs:comment "A clef is a symbol at the beginning of a musical piece that indicates the pitch of the written notes."@en ,
                   "The property relates an incipit to its clef."@en ;
      rdfs:label "clef"@en ;
      <https://nfdi.fiz-karlsruhe.de/ontology/example> "\"G-2\"" .


###  https://nfdi4culture.de/ontology#creationDate
:creationDate rdf:type owl:DatatypeProperty ;
              rdfs:subPropertyOf <http://schema.org/temporalCoverage> ;
              rdfs:domain :Item ;
              rdfs:range [ rdf:type rdfs:Datatype ;
                           owl:unionOf ( xsd:date
                                         xsd:dateTime
                                         xsd:dateTimeStamp
                                       )
                         ] ;
              rdfs:comment "The property relates an item to the exact date when the item was created or came into existence."@en ;
              rdfs:label "creation date"@en ;
              <https://nfdi.fiz-karlsruhe.de/ontology/example> "\"1380-01-01T00:00:00\""^^rdfs:Literal .


###  https://nfdi4culture.de/ontology#creationPeriod
:creationPeriod rdf:type owl:DatatypeProperty ;
                rdfs:subPropertyOf <http://schema.org/temporalCoverage> ;
                rdfs:domain :Item ;
                rdfs:range rdfs:Literal ;
                rdfs:comment "The property links an item to the time period that indicates the time span during which the item was created."@en ;
                rdfs:label "creation period"@en ;
                <https://nfdi.fiz-karlsruhe.de/ontology/example> "\\\"1888\\\", \\\"1380-01-01T00:00:00/1400-12-31T23:59:59\\\", \\\"18-19 Jh\\\""@en .


###  https://nfdi4culture.de/ontology#destructionDate
:destructionDate rdf:type owl:DatatypeProperty ;
                 rdfs:subPropertyOf <http://schema.org/temporalCoverage> ;
                 rdfs:domain :Item ;
                 rdfs:range [ rdf:type rdfs:Datatype ;
                              owl:unionOf ( xsd:date
                                            xsd:dateTime
                                            xsd:dateTimeStamp
                                          )
                            ] ;
                 rdfs:comment "The property relates an item to the specific date on which the item ceases to exist or is intentionally terminated, discarded, or removed."@en ;
                 rdfs:label "destruction date"@en ;
                 <https://nfdi.fiz-karlsruhe.de/ontology/example> "\"1891-07-06T00:00:00\""^^rdfs:Literal .


###  https://nfdi4culture.de/ontology#elementTypeLiteral
:elementTypeLiteral rdf:type owl:DatatypeProperty ;
                    rdfs:domain :DatafeedElement ;
                    rdfs:range rdfs:Literal ;
                    rdfs:comment "The property relates a datafeed element to its broader category, indicating the nature of the element."@en ,
                                 "cto:elementTypeLiteral should only be used when associated item types lack URIs or when the use of cto:elementType is not possible."@en ;
                    rdfs:label "element type literal"@en ;
                    <https://nfdi.fiz-karlsruhe.de/ontology/example> "\"Glaskunst (Objektgattung)\", \"Schauspiel\", \"Fliegende Blätter\", \"Human\""^^rdfs:Literal .


###  https://nfdi4culture.de/ontology#existencePeriod
:existencePeriod rdf:type owl:DatatypeProperty ;
                 rdfs:subPropertyOf <http://schema.org/temporalCoverage> ;
                 rdfs:domain :Item ;
                 rdfs:range rdfs:Literal ;
                 rdfs:comment "The property links an item to the time period that indicates the time span during which the item existed. The property should only be used when the use of cto:creationDate and cto:distructionDate is not possible."@en ;
                 rdfs:label "existence period"@en ;
                 <https://nfdi.fiz-karlsruhe.de/ontology/example> "\"17 Jahrhundert\", \"1890s\""@en .


###  https://nfdi4culture.de/ontology#keySignature
:keySignature rdf:type owl:DatatypeProperty ;
              rdfs:domain :Incipit ;
              rdfs:range rdfs:Literal ;
              rdfs:comment "A key signature is a set of sharp or flat symbols placed on the staff at the beginning of a piece of music, indicating the key of the composition."@en ,
                           "The property relates an incipit to its key signature."@en ;
              rdfs:label "key signature"@en ;
              <https://nfdi.fiz-karlsruhe.de/ontology/example> "\"xF\""^^rdfs:Literal .


###  https://nfdi4culture.de/ontology#pattern
:pattern rdf:type owl:DatatypeProperty ;
         rdfs:domain :Incipit ;
         rdfs:range rdfs:Literal ;
         rdfs:comment "A pattern of an incipit refers to an initial sequence of notes, chords, or rhythms."@en ,
                      "The property relates an incipit to its pattern."@en ;
         rdfs:label "pattern"@en ;
         <https://nfdi.fiz-karlsruhe.de/ontology/example> "\"4'D/8.6GB4AG/8.6''EC2'A/4.''D8'BAG/4BA\""^^rdfs:Literal .


###  https://nfdi4culture.de/ontology#relatedEventLiteral
:relatedEventLiteral rdf:type owl:DatatypeProperty ;
                     rdfs:domain :DatafeedElement ;
                     rdfs:range rdfs:Literal ;
                     rdfs:comment "The property relates an element to events related to the element in a textual or non-URI-based representation."@en ,
                                  "cto:relatedEventLiteral should only be used when associated organizations lack URIs or when the use of cto:relatedEvent is not possible."@en ;
                     rdfs:label "related event literal"@en .


###  https://nfdi4culture.de/ontology#relatedLocationLiteral
:relatedLocationLiteral rdf:type owl:DatatypeProperty ;
                        rdfs:domain :DatafeedElement ;
                        rdfs:range rdfs:Literal ;
                        rdfs:comment "The property relates a datafeed element to locations associated with the described element in a textual or non-URI-based representation."@en ,
                                     "cto:relatedLocationLiteral should only be used when associated locations lack URIs or when the use of cto:relatedLocation is not possible."@en ;
                        rdfs:label "related location literal"@en ;
                        <https://nfdi.fiz-karlsruhe.de/ontology/example> "\"Abtei Altenberg\", \"Berlin\""^^rdfs:Literal .


###  https://nfdi4culture.de/ontology#relatedOrganizationLiteral
:relatedOrganizationLiteral rdf:type owl:DatatypeProperty ;
                            rdfs:domain :DatafeedElement ;
                            rdfs:range rdfs:Literal ;
                            rdfs:comment "The property relates an element to organizations related to the element in a textual or non-URI-based representation."@en ,
                                         "cto:relatedOrganizationLiteral should only be used when associated organizations lack URIs or when the use of cto:relatedOrganization is not possible."@en ;
                            rdfs:label "related organization literal"@en .


###  https://nfdi4culture.de/ontology#relatedPersonLiteral
:relatedPersonLiteral rdf:type owl:DatatypeProperty ;
                      rdfs:domain :DatafeedElement ;
                      rdfs:range rdfs:Literal ;
                      rdfs:comment "The property relates a datafeed element to individuals associated with the described element in a textual or non-URI-based representation."@en ,
                                   "cto:relatedPersonLiteral should only be used when associated persons lack URIs or when the use of cto:relatedPerson is not possible."@en ;
                      rdfs:label "related person literal"@en ;
                      <https://nfdi.fiz-karlsruhe.de/ontology/example> "\"Felix Cziossek\""^^rdfs:Literal .


###  https://nfdi4culture.de/ontology#subjectConceptLiteral
:subjectConceptLiteral rdf:type owl:DatatypeProperty ;
                       rdfs:domain :DatafeedElement ;
                       rdfs:range rdfs:Literal ;
                       rdfs:comment "The property relates an element to concepts related to the subject of the element in a textual or non-URI-based representation."@en ,
                                    "cto:subjectConceptLiteral should only be used when associated concepts lack URIs or when the use of cto:subjectConcept is not possible."@en ;
                       rdfs:label "subject concept literal"@en ;
                       <https://nfdi.fiz-karlsruhe.de/ontology/example> "\"Coro\", \"Monumente\""^^rdfs:Literal .


###  https://nfdi4culture.de/ontology#timeSignature
:timeSignature rdf:type owl:DatatypeProperty ;
               rdfs:domain :Incipit ;
               rdfs:range rdfs:Literal ;
               rdfs:comment "A time signature is a notation convention that indicates the number of beats in each measure and which note value represents one beat."@en ,
                            "The property relates an incipit to its time signature."@en ;
               rdfs:label "time signature"@en ;
               <https://nfdi.fiz-karlsruhe.de/ontology/example> "\"3/4\", \"4/4\""^^rdfs:Literal .


#################################################################
#    Classes
#################################################################

###  http://purl.org/ontology/mo/Lyrics
<http://purl.org/ontology/mo/Lyrics> rdf:type owl:Class .


###  http://purl.org/ontology/mo/MusicalWork
<http://purl.org/ontology/mo/MusicalWork> rdf:type owl:Class ;
                                          owl:equivalentClass <http://schema.org/MusicComposition> .


###  http://schema.org/CreativeWork
<http://schema.org/CreativeWork> rdf:type owl:Class ;
                                 owl:equivalentClass :Item .


###  http://schema.org/MediaObject
<http://schema.org/MediaObject> rdf:type owl:Class ;
                                rdfs:subClassOf <http://schema.org/CreativeWork> .


###  http://schema.org/MusicComposition
<http://schema.org/MusicComposition> rdf:type owl:Class ;
                                     rdfs:subClassOf <http://schema.org/CreativeWork> .


###  https://nfdi.fiz-karlsruhe.de/ontology/Event
<https://nfdi.fiz-karlsruhe.de/ontology/Event> rdf:type owl:Class .


###  https://nfdi.fiz-karlsruhe.de/ontology/Organization
<https://nfdi.fiz-karlsruhe.de/ontology/Organization> rdf:type owl:Class .


###  https://nfdi.fiz-karlsruhe.de/ontology/Person
<https://nfdi.fiz-karlsruhe.de/ontology/Person> rdf:type owl:Class .


###  https://nfdi.fiz-karlsruhe.de/ontology/Place
<https://nfdi.fiz-karlsruhe.de/ontology/Place> rdf:type owl:Class .


###  https://nfdi.fiz-karlsruhe.de/ontology/Resource
<https://nfdi.fiz-karlsruhe.de/ontology/Resource> rdf:type owl:Class .


###  https://nfdi4culture.de/ontology#DatafeedElement
:DatafeedElement rdf:type owl:Class ;
                 rdfs:subClassOf <https://nfdi.fiz-karlsruhe.de/ontology/Resource> ;
                 rdfs:comment "A datafeed element refers to an individual data point or entry within a larger dataset."@en ,
                              "Datafeed element"@en ,
                              """DatafeedElement serves to signify membership within a particular resource or datafeed. Thus, entities of various types—such as of types nfdicore:Person, nfdicore:Place, cto:Item, or nfdicore:Event, etc. may acquire the additional designation of DatafeedElement if they are included in e.g. a dataset and are described within the graph.

The recommended properties to describe datafeed elements: 

cto:elementOf
nfdicore:publisher
nfdicore:license
schema:url
cto:elementType
cto:subjectConcept
cto:relatedPerson
cto:relatedItem
cto:relatedEvent
cto:relatedOrganisation
cto:relatedLocation
cto:externalVocabulary
schema:temporalCoverage"""@en .


###  https://nfdi4culture.de/ontology#Incipit
:Incipit rdf:type owl:Class ;
         rdfs:subClassOf <http://schema.org/CreativeWork> ;
         rdfs:comment "A resource that represents an opening segment of a music composition."@en ;
         rdfs:label "Incipit"@en ;
         <https://nfdi.fiz-karlsruhe.de/ontology/example> "https://rism.online/sources/201001959/incipits/1.1.1"@en .


###  https://nfdi4culture.de/ontology#Item
:Item rdf:type owl:Class ;
      rdfs:comment "A creative work that represents a discrete, identifiable item within diverse resources, e.g. individual artwork in a collection, a record in a dataset, etc."@en ,
                   "item is a subclass of \\\"schema:CreativeWork\\\", indicating that all items inherently fall under the umbrella of creative works. However, for more refined classification, one can employ more specific subclasses of \\\"schema:CreativeWork,\\\" such as \\\"schema:VisualArtwork,\\\" \\\"schema:Photograph,\\\" or \\\"schema:MusicComposition,\\\" to better define the RDF type of an item and achieve a more granular level of categorization."@en ;
      rdfs:label "Item"@en ;
      <https://nfdi.fiz-karlsruhe.de/ontology/example> "A photograph of the stone sword Matū Ajimā Mandira, a single theatrical performance of \"Was ihr Wollt\" staged on March 11, 1923, a musical composition \"Frühlingsgruß\", a stained glass window artwork \"Engel mit Dudelsack\", a page from a satirical magazine featuring a poem and a caricature image titled \"Gedichte eines Kleinstädters\" ."@en .


###  Generated by the OWL API (version 5.1.18) https://github.com/owlcs/owlapi/
